\documentclass[12pt, a4paper]{amsart}

\usepackage{amsmath, amsthm, amssymb}
\usepackage[top=3cm,right=2.5cm,bottom=3cm,left=2.5cm]{geometry}

\usepackage{lmodern}
\usepackage{pxfonts}

\newcommand{\Exp}{\operatorname{Exp}}
\newcommand{\id}{\operatorname{id}}
\newcommand{\g}{\mathfrak}
\newcommand{\ad}{\operatorname{ad}}
\newcommand{\Ad}{\operatorname{Ad}}
\newcommand{\Span}{\operatorname{span}}
\newcommand{\R}{\mathbb{R}}
\newcommand{\C}{\mathbb{C}}
\renewcommand{\H}{\mathbb{H}}
\renewcommand{\Re}{\operatorname{Re}}
\renewcommand{\Im}{\operatorname{Im}}
\newcommand{\Sp}{\mathsf{Sp}}

\newtheorem{theorem}{Theorem}[section]
\newtheorem{proposition}[theorem]{Proposition}
\newtheorem{lemma}[theorem]{Lemma}
\theoremstyle{remark}
\newtheorem*{remark}{Remark}

\begin{document}
\title{Quaternionic projective spaces}

\begin{abstract}
We present the construction and some properties of quaternionic projective and hyperbolic spaces.
\end{abstract}

\date{\today}
\maketitle

\section{Quaternions}

Quaternions are a normed real division algebra,  
{$\H=\{t+\mathbf{i}x+\mathbf{j}y+\mathbf{k}z:t,x,y,z\in\R\}$}, that can be understood as the vector space $\R^4$. 
Product consists in applying asociative and distributive properties to expressions as before, 
taking into account that $\mathbf{i}^2=\mathbf{j}^2=\mathbf{k}^2=-1$, $\mathbf{i}\mathbf{j}=\mathbf{k}=-\mathbf{j}\mathbf{i}$, and real numbers commute with the symbols 
$\mathbf{i}$, $\mathbf{j}$, $\mathbf{k}$. 
Product is associative, has identity element $1$, and any element has an inverse.

Let $q=t+\mathbf{i}x+\mathbf{j}y+\mathbf{k}z$ be a quaternion. 
The real or scalar part is $\Re{q}=t$ and the imaginary or vector part is 
$\Im{q}=\mathbf{i}x+\mathbf{j}y+\mathbf{k}z$. 
The {conjugate} of $q$ is the quaternion $\overline{q}=t-\mathbf{i}x-\mathbf{j}y-\mathbf{k}z$. 
We have $\overline{q_1 q_2}=\overline{q_2}\,\overline{q_1}$. 
The absolute value or norm of a quaternion is given by
$\lvert q\rvert^2=q\overline{q}=\overline{q}q=t^2+x^2+y^2+z^2$, 
which is the same as the usual norm of $\R^4$. 
An important fact is that norm is multiplicative, that is,
$\lvert pq\rvert=\lvert p\rvert\lvert q\rvert$ for all $p$,~$q\in\H$. 
Moreover, if $q\neq 0$ we have $q^{-1}=\frac{\overline{q}}{\lvert q\rvert^2}$.

The quaternion product is determined by the following rules:
\begin{itemize}
\item $\Re{(q_1 q_2)}=(\Re{q_1})(\Re{q_2})-\langle \Im{q_1},\Im{q_2}\rangle$,
\item $\Im{(q_1 q_2)}=(\Re{q_1})(\Im{q_2})+(\Re{q_2})(\Im{q_1})+\Im{q_1}\times\Im{q_2}$,
\end{itemize}
where $\langle\cdot,\cdot\rangle$ is the scalar product of $\R^3\cong\Im\H$, 
and $\cdot\times\cdot$ is the vector product. 

With the identification $\Im\H\cong\R^3$, and if $\{\mathbf{i},\mathbf{j},\mathbf{k}\}$ is identified with the canonical basis of $\R^3$ then, for any $q_1$, $q_2\in\Im{\H}\cong\R^3$, we have $q_1 q_2=-\langle q_1,q_2\rangle+q_1\times q_2$.

From the equations above, if $\lambda\in\H$ is such that $q\lambda=\lambda q$ for any $q\in\H$, then $\lambda\in\R$.

\begin{remark}
We define $\Sp(1)=\{q\in\H:\lvert q\rvert =1\}$.
We consider $\varphi\colon\Sp(1)\to\mathsf{SO}(\Im\H)$, given by $\varphi(q)(x)=qxq^{-1}$. 
The map $\varphi(q)$ is isometric because $\lvert\varphi(q)(x)\rvert=\lvert qxq^{-1}\rvert=\lvert x\rvert$. 
If $\lambda\in\R$ then $\varphi(q)(\lambda)=q\lambda q^{-1}=\lambda$, so $\varphi(q)(\R)=\R$, and thus, $\varphi(q)(\Im\H)=\Im\H$. 
Hence, $\varphi(\Sp(1))\subset\mathsf{O}(\Im\H)$.
Since $\Sp(1)$ is connected, $\det\varphi(\Sp(1))=1$. 
As a consequence, $\varphi(\Sp(1))\subset\mathsf{SO}(\Im\H)$ and this map is well-defined.
Furthermore, $\varphi$ is clearly a Lie group homomorphism because $\mathsf{SO}(\Im\H)$ is a closed subgroup of $\mathsf{GL}(\Im\H)$. 

The Lie algebra $\g{sp}(1)$ of $\Sp(1)$ can be identified with $\Im\H$.
For $u\in\Im\H$ and $t\in\R$ we define $e^{tu}=\cos t+u\sin t$.
Then, 
\[
\varphi_{*1}(u)(v)=\frac{d}{dt}\bigg\vert_0\varphi(e^{tu})v=uv-vu=2(u\times v).
\]
This map is clearly an isomorphism of Lie algebras. 
Therefore, $\varphi$ is a covering of Lie groups.
Moreover, it follows easily that $\ker\varphi={\pm 1}$, and hence, $\mathsf{SO}(3)=\Sp(1)/\mathbb{Z}_2\cong\R\mathsf{P}^3$.
\end{remark}

\section{Quaternionic vector spaces}

A quaternionic vector space is, in fact, a right $\H$-module.

Let $V$ and $W$ be two quaternion vector spaces. 
A map $L\colon V\to W$ is $\H$-linear if $L(\mathbf{v}q)=L(\mathbf{v})q$ for ach $\mathbf{v}\in V$ and $q\in\H$. Let $\{\mathbf{v}_1,\dots,\mathbf{v}_n\}$ be a basis of $V$ and $\{\mathbf{w}_1,\dots,\mathbf{w}_m\}$ a basis of $W$. 
We may write $L(\mathbf{v}_j)=\sum_i \mathbf{w}_i a_{ij}$, with $a_{ij}\in\H$. 
If $\mathbf{v}=\sum_j \mathbf{v}_j\lambda_j\in V$, $\lambda_j\in\H$ we have 
\[
L(\mathbf{v})
=L\Bigl(\sum_j \mathbf{v}_j\lambda_j\Bigr)
=\sum_j L(\mathbf{v}_j)\lambda_j{}=\sum_j\Bigl(\sum_i \mathbf{w}_i a_{ij}\Bigr)\lambda_j
=\sum_{i}\mathbf{w}_i\Bigl(\sum_j a_{ij}\lambda_j\Bigr),
\]
so the coordinates of $L(\mathbf{v})$ with respect to $\{\mathbf{w}_1,\dots,\mathbf{w}_m\}$ are given by
\[
\begin{pmatrix}
a_{11} & \cdots & a_{1n}\\
\vdots & \ddots & \vdots\\
a_{m1} & \cdots & a_{mn}
\end{pmatrix}
\begin{pmatrix}
\lambda_1\\
\vdots\\
\lambda_n
\end{pmatrix}.
\]
With this convention, composition of $\H$-linear maps corresponds to multiplication of quaternion matrices.

A quaternion product is a map $(\,\cdot\,,\,\cdot\,\,)\colon V\times V\to\H$ such that:
\begin{enumerate}
\item $(\mathbf{x}+\mathbf{y},\mathbf{z})
=(\mathbf{x},\mathbf{z})+(\mathbf{y},\mathbf{z})$,
$(\mathbf{x},\mathbf{y}+\mathbf{z})
=(\mathbf{x},\mathbf{y})+(\mathbf{x},\mathbf{z})$,
\item $(\mathbf{x}q,\mathbf{y})=\overline{q}(\mathbf{x},\mathbf{y})$, $(\mathbf{x},\mathbf{y}q)=(\mathbf{x},\mathbf{y}) q$,
\item $(\mathbf{x},\mathbf{y})=\overline{(\mathbf{y},\mathbf{x})}$,
\item $(\mathbf{x},\mathbf{x})\geq 0$, with equality if and only if $\mathbf{x}=\mathbf{0}$,
\end{enumerate}
for all $\mathbf{x}$, $\mathbf{y}$, $\mathbf{z}\in V$, $q\in H$.

Note that $\langle\mathbf{x},\mathbf{y}\rangle=\Re(\mathbf{x},\mathbf{y})$ defines an inner product in $V$.

In particular, $\H^n$ is quaternion vector space and $(\mathbf{x},\mathbf{y})=\sum_{i=1}^n \overline{x_i}y_i$ defines a quaternion product on $\H^n$. The usual scalar product of $\R^{4n}\cong\H^n$ coincides with $\langle\mathbf{x},\mathbf{y}\rangle=\Re(\mathbf{x},\mathbf{y})$.


We define the general quaternion linear group $\mathsf{GL}(n,\H)$ as the group of invertible quaternion matrices; it is isomorphic with the group of invertible $\H$-linear endomorphisms of $\H^n$. 
The symplectic group is defined as $\Sp(n)=\{A\in\mathsf{GL}(n,\H):A^* A=\id\}$.
This group coincides with the group of quaternion matrices that preserve the quaternion product of $\H^n$.	

\medskip

Let $V$ be a real vector space with inner product $\langle\,\cdot\,,\,\cdot\,\rangle$.
A $3$-dimensional subspace $\g{q}$ of $\g{so}(V)$ is called a linear quaternionic structure if there are elements $J_1$, $J_2$, $J_3\in\g{q}$ such that $J_i^2=-1$ and $J_iJ_{i+1}=J_{i+2}$ (indices modulo 3).
Then, $\g{q}$ is a subalgebra of $\g{so}(V)$ isomorphic to $\g{sp}(1)$.

If $V$ is a quaternionic vector space with a quaternionic product as above, we define $J_1(\mathbf{x})=-\mathbf{x}\mathbf{i}$, $J_2(\mathbf{x})=-\mathbf{x}\mathbf{j}$, $J_3(\mathbf{x})=-\mathbf{x}\mathbf{k}$.
Then, $\g{q}=\R J_1\oplus\R J_2\oplus\R J_3$ is a linear quaternionic structure on $V$.

\begin{proof}
For example,
\[
J_1 J_2(\mathbf{v})
=J_1(-\mathbf{v}\mathbf{j})
=\mathbf{v}\mathbf{j}\mathbf{i}
=-\mathbf{v}\mathbf{k}
=J_3(\mathbf{v}).
\]
We also show as an example,
\begin{align*}
\langle J_1\mathbf{v},J_1\mathbf{w}\rangle
&{}=\langle -\mathbf{v}\mathbf{i},-\mathbf{v}\mathbf{i}\rangle
=\Re (\mathbf{v}\mathbf{i},\mathbf{v}\mathbf{i})\\
&{}=\Re -\mathbf{i} (\mathbf{v},\mathbf{w}) \mathbf{i}
=\Re (\mathbf{v},\mathbf{w}) (-\mathbf{i}\mathbf{i})
=\Re (\mathbf{v},\mathbf{w})
=\langle \mathbf{v},\mathbf{w}\rangle.\qedhere
\end{align*}
\end{proof}

Conversely, if $\g{q}$ is a linear quaternionic structure on $V$, then we can define a right quaternionic vector space structure on $V$ as $\mathbf{v}(t+x\mathbf{i}+y\mathbf{j}+z\mathbf{k})=t\mathbf{v}+xJ_1(\mathbf{v})+yJ_2(\mathbf{v})+zJ_3(\mathbf{v})$.

\begin{proof}
For example, we check
\[
\begin{aligned}
\mathbf{v}\mathbf{i}\mathbf{j}
=J_1(\mathbf{v})\mathbf{j}
=J_2 J_1(\mathbf{v})
=-J_1 J_2(\mathbf{v})
=-J_3(\mathbf{v})
=\mathbf{v}\mathbf{k}.
\end{aligned} \qedhere
\]
\end{proof}

\section{Quaternionic projective spaces}

Let $V$ be a quaternion vector space of quaternionic dimension $n+1$ endowed with a quaternion product $(\,\cdot\,,\,\cdot\,\,)$, and $\langle\,\cdot\,,\,\cdot\,\,\rangle=\Re(\,\cdot\,,\,\cdot\,\,)$.
Then $V$ is isomorphic with $\H^{n+1}$ with the usual quaternion product.

We consider the sphere $\mathsf{S}^{4n+3}=\mathsf{S}(V)=\{{x}\in V:\langle {x},{x}\rangle=1\}$.
We define the right action $\mathsf{S}(V)\times\Sp(1)\to\mathsf{S}(V)$ by ${x}\cdot \lambda={x}\lambda$.
This action is obviously proper and free. 
Hence, the orbit space 
\[
\mathsf{P}(V)=\mathsf{S}(V)/\Sp(1)
\]
is a smooth manifold of real dimension $4n$, that is called the quaternion projective space of $V$.
If $V=\H^{n+1}$, then we denote this space by $\H \mathsf{P}^n$.

We denote by $\pi\colon\mathsf{S}(V)\to\mathsf{P}(V)$ the quotient map.
This map is a submersion that is called the Hopf map.
If ${x}\in\mathsf{S}(V)$, then we can identify $T_{x}\mathsf{S}(V)=(\R{x})^\perp=V\ominus\R{x}$, the orthogonal complement of ${x}$ with respect to $\langle\,\cdot\,,\,\cdot\,\,\rangle$.
Thus, $\ker\pi_{*{x}}={x}\Im\H$, and we have an orthogonal decomposition 
\[
T_{x}\mathsf{S}(V)=({x}\Im\H)\oplus(\H{x})^\perp.
\]
We endow $\mathsf{P}(V)$ with a Riemannian metric that makes $\pi$ a Riemannian submersion.
Thus, $T_{\pi({x})}\mathsf{P}(V)$ becomes isometric to $(\H{x})^\perp$ through $\pi_{*{x}}$.
A vector in $(\H x)^\perp$ is called horizontal, and a vector in $\ker\pi_{*x}$ is called vertical, as it is common for Riemannian submersions~\cite{ONeill}.

Let $v\in T_{p}\mathsf{P}(V)$.
For ${x}\in\pi^{-1}(p)$ we define the horizontal lift $v^L_{x}$ of $v$ as the unique vector $v_x^L\in(\H{x})^\perp$ such that $\pi_{*{x}}(v^L_{x})=v$.
Note that, with the usual identifications, we have $v_{x\lambda}^L=v_x^L\lambda$, with $\lambda\in\Sp(1)$, since $(x\Im\H)^\perp$ is $\H$-invariant and $\pi_{x\lambda}(v_x^L\lambda)=\pi_{*x}(v_x^L)$.
\medskip

In order to give $\mathsf{P}(V)$ a structure of Riemannian manifold, we require $\pi$ to be a Riemannian submersion.
This implies that the metric on $\mathsf{P}(V)$ is defined as 
\[
\langle v,w\rangle_{\mathsf{P}(V)}=\langle v^L,w^L\rangle_{\mathsf{S}(V)}
\] 
for each $v$, $w\in T_p\mathsf{P}(V)$.
We will omit subindices whenever the space where were considering the Riemannian metric is clear.
We see that this definition does not depend on the point ${x}\in\pi^{-1}(p)$ used to define the lift.
Indeed,
\[
\langle v^L_{{x}\lambda},w^L_{{x}\lambda}\rangle=
\langle v^L_{{x}}\lambda,w^L_{{x}}\lambda\rangle=
\Re\bar{\lambda}(v^L_{x},w^L_{x})\lambda=
\Re\lvert\lambda\rvert^2(v^L_{x},w^L_{x})=
\langle v^L_{x},w^L_{x}\rangle.
\]

Since $\pi\colon\mathsf{S}(V)\to\mathsf{P}(V)$ is a Riemannian submersion, the Levi-Civita connection $\nabla$ of $\mathsf{P}(V)$ is determined by~\cite{ONeill}
\[
(\nabla_X Y)_{\pi(x)}=\pi_{*x}(\tilde{\nabla}_X Y),
\]
where $\tilde{\nabla}$ is the Levi-Civita connection of $\mathsf{S}(V)$.
\medskip

Now we define a quaternion K\"ahler structure on $\mathsf{P}(V)$.

Let $\sigma\colon U\to\mathsf{S}(V)$ be a section of $\pi$, that is, a smooth map such that $\pi\circ\sigma=\id$ in the open set $U$ of $\mathsf{P}(V)$.
We define, for $X\in\Gamma(T\mathsf{P}(V))$,
\[
\begin{aligned}
J_1(X_p)&{}=\pi_{*\sigma(p)}(-X_{\sigma(p)}^L\mathbf{i}),
&J_2(X_p)&{}=\pi_{*\sigma(p)}(-X_{\sigma(p)}^L\mathbf{j}),
&J_3(X_p)&{}=\pi_{*\sigma(p)}(-X_{\sigma(p)}^L\mathbf{k}),
\end{aligned}
\]
for $p\in U$.
The same definition can be made for $v\in T_p\mathsf{P}(V)$.
It is important to note, however, that this definition depends on the choice of section $\sigma$.

\begin{lemma}
The above definition determines a quaternionic K\"ahler structure on $\mathsf{P}(V)$.
\end{lemma}

\begin{proof}
In order to shorten the notation we define $\mathcal{V}=\ker\pi_{*\sigma(p)}=\sigma(p)\Im\H$, and $\mathcal{V}^\perp$ its quaternionic orthogonal complement.
Note that ${\mathcal{V}}^\perp$ is $\H$-invariant, a fact that we will use often in this proof.

First we check that $J_i^2=-\id$.
For example, 
\[
\begin{aligned}
J_1^2(X_p)
=J_1(\pi_{*\sigma(p)}(-X_{\sigma(p)}^L\mathbf{i}))
=\pi_{*\sigma(p)}(X_{\sigma(p)}^L\mathbf{i}\mathbf{i})
=-X_p,
\end{aligned}
\]
using that $\mathcal{V}^\perp$ is $\H$-invariant, and this, multiplication by $\mathbf{i}$ maps horizontal vectors to horizontal vectors.

Similarly,
\[
\begin{aligned}
J_1 J_2(X_p)
=J_1(\pi_{*\sigma(p)}(-X_{\sigma(p)}^L\mathbf{j}))
=\pi_{*\sigma(p)}(X_{\sigma(p)}^L\mathbf{j}\mathbf{i})
=\pi_{*\sigma(p)}(-X_{\sigma(p)}^L\mathbf{k})
=J_3(X_p).
\end{aligned}
\]

Since $\pi$ is a Riemannian submersion,
\[
\begin{aligned}
\langle J_1(X_p),J_1(Y_p)\rangle
=\langle \pi_{*\sigma(p)}(-X_{\sigma(p)}^L\mathbf{i}),\pi_{*\sigma(p)}(-Y_{\sigma(p)}^L\mathbf{i})\rangle
=\langle X_{\sigma(p)}^L\mathbf{i}, Y_{\sigma(p)}^L\mathbf{i}\rangle
=\langle X_{\sigma(p)}^L, Y_{\sigma(p)}^L\rangle
=\langle X_p,Y_p\rangle.
\end{aligned}
\]

Now we show that the space $\g{q}$ generated by $\{J_1,J_2,J_3\}$ is invariant with respect to the Levi-Civita connection, that is, $\nabla_X\g{q}\subset\g{q}$.
To that end we calculate $(\nabla_X J_1)_p Y$, $p\in \mathsf{P}(V)$, $X$, $Y\in\Gamma(TU)$.

Let $\gamma\colon I\to U$ be a smooth curve such that $\gamma(0)=p$, $\gamma'(0)=X_p$.
We denote by $\tilde{\gamma}$ its horizontal lift to $\sigma(U)\subset\mathsf{S}(V)$ through $\sigma(p)$.
Thus, $\tilde{\gamma}(0)=\sigma(p)$, $\tilde{\gamma}'(0)=X_p^L$.
We write $\tilde{\gamma}(t)=\sigma(\gamma(t))\lambda(t)$, where $\lambda$ is a smooth function in $\Sp(1)$.
Since $\sigma(p)=\tilde{\gamma}(0)=\sigma(p)\lambda(0)$ we get $\lambda(0)=1$ and $\lambda'(0)\in T_1\Sp(1)=\Im\H$.

Recall that $\sigma(p)^\perp=T_{\sigma(p)}\mathsf{S}(V)$. In what follows subspaces of $\sigma(p)^\perp$ written as subindices mean orthogonal projection to that subspace.
Recall that $\tilde{\nabla}$ is the Levi-Civita connection of $\mathsf{S}(V)$.
We also denote by $D$ the usual connection of $\H^{n+1}$.

On the one hand,
\[
\begin{aligned}
\nabla_{X_p}(J_1 Y)
&{}=\pi_{*\sigma(p)}\Bigl(\tilde{\nabla}_{X_{\sigma(p)}^L}(J_1 Y)^L\Bigr)
=\pi_{*\sigma(p)}\Bigl(\Bigl(D_{X_{\sigma(p)}^L}(J_1 Y)^L\Bigr)_{\sigma(p)^\perp}\Bigr)\\
&{}=\pi_{*\sigma(p)}\left(
\left(\frac{d}{dt}\Big\vert_0 (J_1 Y)_{\tilde{\gamma}(t)}^L\right)_{\sigma(p)^\perp}\right)
=\pi_{*\sigma(p)}\left(
\left(\frac{d}{dt}\Big\vert_0 (J_1 Y)_{\sigma(\gamma(t))\lambda(t)}^L\right)_{\sigma(p)^\perp}\right)\\
&{}=\pi_{*\sigma(p)}\left(
\left(\frac{d}{dt}\Big\vert_0 (J_1 Y)_{\sigma(\gamma(t))}^L\lambda(t)\right)_{\sigma(p)^\perp}\right)
=\pi_{*\sigma(p)}\left(
\left(-\frac{d}{dt}\Big\vert_0 Y_{\sigma(\gamma(t))}^L\mathbf{i}\lambda(t)\right)_{\sigma(p)^\perp}\right)\\
&{}=\pi_{*\sigma(p)}\left(
-\left(\frac{d(Y^L\circ\sigma\circ\gamma)}{dt}(0)\,\mathbf{i}\lambda(0) +Y_{\sigma(\gamma(0))}^L\mathbf{i}\lambda'(0)\right)_{\sigma(p)^\perp}\right)\\
&{}=\pi_{*\sigma(p)}\left(
-\left(\frac{d(Y^L\circ\sigma\circ\gamma)}{dt}(0)\,\mathbf{i}\right)_{\mathcal{V}^\perp} -Y_{\sigma(p)}^L\mathbf{i}\lambda'(0)\right).
\end{aligned}
\]
On the other hand,
\[
\begin{aligned}
J_1(\nabla_{X_p}Y)
&{}=\pi_{*\sigma(p)}\Bigl(-(\nabla_X Y)_{\sigma(p)}^L\mathbf{i}\Bigr)
=\pi_{*\sigma(p)}\Bigl(
-\Bigl(\pi_{*\sigma(p)}(\tilde{\nabla}_{X_{\sigma(p)}}^L Y^L)\Bigr)_{\sigma(p)}^L\mathbf{i}\Bigr)\\
&{}=\pi_{*\sigma(p)}\Bigl(
-\Bigl(\tilde{\nabla}_{X_{\sigma(p)}}^L Y^L\Bigr)_{\mathcal{V}^\perp}\mathbf{i}\Bigr)
=\pi_{*\sigma(p)}\left(
-\left(\frac{d}{dt}\Big\vert_0 Y_{\tilde{\gamma}(t)}^L\right)_{\mathcal{V}^\perp}\mathbf{i}\right)\\
&{}=\pi_{*\sigma(p)}\left(
-\left(\frac{d}{dt}\Big\vert_0  Y_{\sigma(\gamma(t))\lambda(t)}^L\right)_{\mathcal{V}^\perp}\mathbf{i}\right)
=\pi_{*\sigma(p)}\left(
-\left(\frac{d}{dt}\Big\vert_0  Y_{\sigma(\gamma(t))}^L\lambda(t)\right)_{\mathcal{V}^\perp}\mathbf{i}\right)\\
&{}=\pi_{*\sigma(p)}\left(
-\left(\frac{d(Y^L\circ\sigma\circ\gamma)}{dt}(0)\lambda(0) +Y_{\sigma(\gamma(0))}^L\lambda'(0)\right)_{\mathcal{V}^\perp}\mathbf{i}\right)\\
&{}=\pi_{*\sigma(p)}\left(
-\left(\frac{d(Y^L\circ\sigma\circ\gamma)}{dt}(0)\right)_{\mathcal{V}^\perp}\mathbf{i} -Y_{\sigma(p)}^L\lambda'(0)\mathbf{i}\right).
\end{aligned}
\]
Now we take into account that for any $v\in T_p\mathsf{S}(V)$ we have 
$(v\mathbf{i})_{\mathcal{V}^\perp}=(v_{\mathcal{V}^\perp})\mathbf{i}$, since $\mathcal{V}^\perp$ is $\H$-invariant, to get
\[
\begin{aligned}
(\nabla_{X_p}J_1)Y
=\nabla_{X_p}(J_1 Y)-J_1(\nabla_{X_p}Y)
=\pi_{*\sigma(p)}\bigl(Y_{\sigma(p)}^L[\lambda'(0),\mathbf{i}]\bigr).
\end{aligned}
\]

Recall from the definition of $\lambda$ that 
$X_{\sigma(p)}^L=\tilde{\gamma}'(0)=\sigma_{*p}(X_p)+\sigma(p)\lambda'(0)$.
Thus, we define, taking into account that $X_{\sigma(p)}^L$ is horizontal,
\[
\begin{aligned}
q_1(X)&{}=\frac{1}{2}\langle\sigma_{*p}(X_p),\sigma(p)\mathbf{i}\rangle
=-\frac{1}{2}\langle \sigma(p)\lambda'(0),\sigma(p)\mathbf{i}\rangle
=-\frac{1}{2}\langle \lambda'(0),\mathbf{i}\rangle,\\
q_2(X)&{}=\frac{1}{2}\langle\sigma_{*p}(X_p),\sigma(p)\mathbf{j}\rangle
=-\frac{1}{2}\langle \sigma(p)\lambda'(0),\sigma(p)\mathbf{j}\rangle
=-\frac{1}{2}\langle \lambda'(0),\mathbf{j}\rangle,\\
q_3(X)&{}=\frac{1}{2}\langle\sigma_{*p}(X_p),\sigma(p)\mathbf{k}\rangle
=-\frac{1}{2}\langle \sigma(p)\lambda'(0),\sigma(p)\mathbf{k}\rangle
=-\frac{1}{2}\langle \lambda'(0),\mathbf{k}\rangle,
\end{aligned}
\]
where the last inner product is the standard inner product of $\R^3\equiv\Im\H$.

The bracket relations of the Lie algebra $\g{sp}(1)=\Im\H$ imply
\[
[\lambda'(0),\mathbf{i}]
=2\langle\lambda'(0),\mathbf{k}\rangle\,\mathbf{j}-2\langle\lambda'(0),\mathbf{j}\rangle\,\mathbf{k}.
\]
This implies,
\[
\begin{aligned}
(\nabla_{X_p}J_1)Y
&{}=\pi_{*\sigma(p)}\bigl(Y_{\sigma(p)}^L(2\langle\lambda'(0),\mathbf{k}\rangle\,\mathbf{j}-2\langle\lambda'(0),\mathbf{j}\rangle\,\mathbf{k})\bigr)
=-q_3(X)J_2 Y+q_2(X)J_3 Y.
\end{aligned}
\]

With a similar argument we can get $\nabla_X J_i=-q_{i+2}(X)J_{i+1}+q_{i+1}(X)J_{i+2}$, indices modulo~3, from where the result follows.
\end{proof}

Finally we show

\begin{proposition}
$\mathsf{P}(V)$ has constant quaternionic sectional curvature $4$.
\end{proposition}

\begin{proof}
Let $p\in\mathsf{P}(V)$.
We have to show that any $2$-plane in a quaternionic line of $T_p\mathsf{P}(V)$ has the same sectional curvature.
As usual we denote orthogonal projection onto $\mathcal{V}=\ker\pi_*$ by a subindex.

Let $N$ be the unit normal vector field of the sphere $N_x=x$, for $x\in\mathsf{S}(V)$.
First we calculate, for $X$, $Y\in\Gamma(T\mathsf{P}(V))$ and $\lambda\in\Sp(1)$,
\[
\begin{aligned}
\langle \tilde{\nabla}_{X^L} Y^L,N\lambda\rangle
=-\langle Y^L,D_{X^L}(N\lambda)\rangle
=-\langle Y^L,(D_{X^L}N)\lambda\rangle
=-\langle Y^L,X^L \lambda\rangle
=\langle X^L,Y^L \lambda\rangle.
\end{aligned}
\]

Let $\g{q}$ be a local quaternionic structure as defined above and $J\in\g{q}$ a complex structure.
Let $X\in T_p\mathsf{P}(V)$ with $\lvert X\rvert=1$. 
We have to calculate the sectional curvature of the $2$-plane spanned by $X$ and $JX$, and see that this does not depend on $p$ or $X$.

First we have 
\[
\langle[X^L,(JX)^L],N\lambda\rangle
=\langle X^L,(JX)^L\lambda\rangle-\langle(JX)^L,X^L\lambda\rangle
=2\langle X^L,(JX)^L\lambda\rangle.
\]
This implies $\lvert[X^L,(JX)^L]_\mathcal{V}\rvert^2=4\lvert X^L\rvert^2$.
Using~\cite[Corollary~1]{ONeill}, the formula above, and since the sphere of radius $1$ has sectional curvature $1$, we get
\[
K(X, JX)
=1+\frac{3}{4}\bigl\lvert[X^L,JX^L]_\mathcal{V}\bigr\rvert^2
=4,
\]
as we wanted to show.
\end{proof}

In $V$ we can consider the action of $\Sp(V)\cong\Sp(n+1)$ on the left as
$A\cdot\mathbf{x}=A\mathbf{x}$, where matrix multiplication is $\H$-linear on the right.
This action leaves the sphere $\mathsf{S}(V)$ invariant because
\[
\langle A\mathbf{x},A\mathbf{x}\rangle
=\Re(A\mathbf{x},A\mathbf{x})
=\Re(\mathbf{x},\mathbf{x})
=\langle \mathbf{x},\mathbf{x}\rangle=1.
\]
Moreover $\pi(A(x\lambda))=\pi((Ax)\lambda)=\pi(Ax)$, so the action descends to $\mathsf{P}(V)$ as $A\cdot\pi(\mathbf{x})=\pi(A\cdot\mathbf{x})$.

The action of $\Sp(V)$ on $\mathsf{P}(V)$ is transitive because $\Sp(V)$ acts transitively on quaternionic lines through the origin.
It is also isometric.
Let $p\in\mathsf{P}(V)$ and $v$, $w\in T_p\mathsf{P}(V)$.
Let $\alpha\colon I\to\mathsf{P}(V)$ be a smooth curve such that $\alpha(0)=p$, $\alpha'(0)=v$.
We select $x\in\pi^{-1}(p)$ and let $\tilde{\alpha}$ be the horizontal lift of $\alpha$ to $\mathsf{S}(V)$.
Then, $\tilde{\alpha}(0)=x$ and $\tilde{\alpha}'(0)=v_x^L$.
Since $A$ acts linearly on $V$ ,
\[
A_{*p}(v)
=\frac{d}{dt}\Big\vert_0 A(\alpha(t))
=\frac{d}{dt}\Big\vert_0 A(\pi(\tilde{\alpha}(t)))
=\frac{d}{dt}\Big\vert_0 \pi(A\tilde{\alpha}(t))
=\pi_{*x}(A\tilde{\alpha}'(0))
=\pi_{*x}(Av_x^L).
\]
Now, since $\pi$ is a Riemannian submersion
\[
\langle A_{*p}(v),A_{*p}w\rangle
=\langle \pi_{*x}(A v_x^L),\pi_{*x}(A w_x^L)\rangle
=\langle A v_x^L,A w_x^L\rangle
=\langle v_x^L,w_x^L\rangle
=\langle v,w\rangle.
\]

The effectivity kernel of $\Sp(V)$ is $\mathbb{Z}_2=\{\pm \id\}$.
Indeed, if $A\in\Sp(V)$ acts as the identity on $\mathsf{P}(V)$, for each $x\in\mathsf{S}(V)$ we have 
$\pi(Ax)=A\pi(x)=\pi(x)$.
Hence, for each $x\in\mathsf{S}(V)$ there exists $\lambda(x)\in\Sp(1)$ such that $Ax=x\lambda(x)$.
It is not hard to see that this implies that $A$ is diagonal;
but since the action of $A$ is on the left and the quaternions that commute with any other element are reals numbers, we get that $A$ is a diagonal matrix with real entries.
Thus, $A=\pm\id$.

Let $\{e_1,\dots,e_{n+1}\}$ be a quaternionic orthonormal basis of $V$.
From now on we fix $o=\pi(e_1)$.
We calculate the isotropy group of $\Sp(V)$ at $o$.
If $A(\pi(e_1))=A(o)=o$ then there exists $\lambda\in\Sp(1)$ such that $Ae_1=e_1\lambda$.
Since $A\in\Sp(V)$ we get $A=\lambda\oplus B$ where $B\in\Sp(W)$, where $W$ is the quaternionic orthogonal complement of $e_1$ in $V$.
Therefore the isotropy group of $\Sp(V)$ at $o$ is isomorphic to $\Sp(1)\times\Sp(n)$.


\begin{thebibliography}{99}
\bibitem{ONeill}
B.~O'Neill: The fundamental equations of a submersion, \textit{Michigan Math.\ J.}\ \textbf{13} (1966), 459--469.
\end{thebibliography}
\end{document}